OpenVM: add proof of equivalence with the source code

Garden/OpenVM/BranchEq/core_expr.v
@@ -6,7 +6,9 @@ Global Instance ImmInstructionIsToRocq : ToRocq.C (ImmInstruction.t Expr.t) := {
   to_rocq self indent :=
     ToRocq.cats [ToRocq.indent indent; "ImmInstruction:"; ToRocq.endl;
       ToRocq.to_rocq self.(ImmInstruction.is_valid) (indent + 2);
+      ToRocq.endl;
       ToRocq.to_rocq self.(ImmInstruction.opcode) (indent + 2);
+      ToRocq.endl;
       ToRocq.to_rocq self.(ImmInstruction.immediate) (indent + 2)
     ];
 }.
@@ -18,17 +20,54 @@ Global Instance AdapterAirContextIsToRocq {NUM_LIMBS : Z} :
       ToRocq.cats [ToRocq.indent (indent + 2); "to_pc:"; ToRocq.endl;
         ToRocq.to_rocq self.(AdapterAirContext.to_pc) (indent + 4)
       ];
+      ToRocq.endl;
       ToRocq.cats [ToRocq.indent (indent + 2); "reads:"; ToRocq.endl;
         ToRocq.to_rocq self.(AdapterAirContext.reads) (indent + 4)
       ];
+      ToRocq.endl;
       ToRocq.cats [ToRocq.indent (indent + 2); "writes:"; ToRocq.endl;
         ToRocq.to_rocq self.(AdapterAirContext.writes) (indent + 4)
       ];
+      ToRocq.endl;
       ToRocq.cats [ToRocq.indent (indent + 2); "instruction:"; ToRocq.endl;
         ToRocq.to_rocq self.(AdapterAirContext.instruction) (indent + 4)
       ]
     ];
 }.
+
+Fixpoint sum_for_in_zero_to_n_starting_from_aux
+    (n : nat)
+    (f : Z -> Expr.t)
+    (start : Expr.t) :
+    Expr.t :=
+  match n with
+  | O => start
+  | S n => Expr.Add (sum_for_in_zero_to_n_starting_from_aux n f start) (f (Z.of_nat n))
+  end.
+
+Definition sum_for_in_zero_to_n_starting_from
+    (N : Z)
+    (f : Z -> Expr.t)
+    (start : Expr.t) :
+    Expr.t :=
+  sum_for_in_zero_to_n_starting_from_aux (Z.to_nat N) f start.
+
+Lemma sum_for_in_zero_to_n_starting_from_eq {p} `{Prime p}
+    (env : Env.t)
+    (N : Z)
+    (f : Z -> Expr.t) (f' : Z -> Z)
+    (start : Expr.t) (start' : Z)
+    (H_f : forall (i : Z),
+      Eval.eval env (f i) = f' i
+    )
+    (H_start : Eval.eval env start = start') :
+  Eval.eval env (sum_for_in_zero_to_n_starting_from N f start) =
+  core_with_monad.sum_for_in_zero_to_n_starting_from N f' start'.
+Proof.
+  unfold sum_for_in_zero_to_n_starting_from, core_with_monad.sum_for_in_zero_to_n_starting_from.
+  set (n := Z.to_nat N); clearbody n.
+  induction n; cbn; intros; scongruence.
+Qed.
 
 Definition eval {NUM_LIMBS : Z}
     (self : BranchEqualCoreAir.t NUM_LIMBS)
@@ -55,35 +94,29 @@ Definition eval {NUM_LIMBS : Z}
   let b : Array.t Var.t NUM_LIMBS := local.(BranchEqualCoreCols.b) in
   let inv_marker : Array.t Var.t NUM_LIMBS := local.(BranchEqualCoreCols.diff_inv_marker) in
 
-  let cmp_eq : Expr.t :=
-    Expr.Add
-      (Expr.Mul
-        (Expr.Var local.(BranchEqualCoreCols.cmp_result))
-        (Expr.Var local.(BranchEqualCoreCols.opcode_beq_flag)))
-      (Expr.Mul
-        (Expr.not (Expr.Var local.(BranchEqualCoreCols.cmp_result)))
-        (Expr.Var local.(BranchEqualCoreCols.opcode_bne_flag))) in
+  let! cmp_eq : Expr.t :=
+    MExpr.pure (
+      Expr.Add
+        (Expr.Mul
+          (Expr.Var local.(BranchEqualCoreCols.cmp_result))
+          (Expr.Var local.(BranchEqualCoreCols.opcode_beq_flag)))
+        (Expr.Mul
+          (Expr.not (Expr.Var local.(BranchEqualCoreCols.cmp_result)))
+          (Expr.Var local.(BranchEqualCoreCols.opcode_bne_flag)))
+    ) in
 
   let! _ :=
-    MExpr.List.fold_left
-      (fun acc i =>
-        let i := Z.of_nat i in
-        MExpr.assert_zero
-          (Expr.Mul cmp_eq (Expr.Sub (Expr.Var (Array.get a i)) (Expr.Var (Array.get b i))))
+    MExpr.for_in_zero_to_n NUM_LIMBS (fun i =>
+      MExpr.assert_zero (
+        Expr.Mul cmp_eq (Expr.Sub (Expr.Var (Array.get a i)) (Expr.Var (Array.get b i)))
       )
-      tt
-      (Lists.List.seq 0 (Z.to_nat NUM_LIMBS)) in
+    ) in
   let sum : Expr.t :=
-    Lists.List.fold_left
-      (fun sum (i : nat) =>
-        let i := Z.of_nat i in
-        Expr.Add sum
-          (Expr.Mul
-            (Expr.Sub (Expr.Var (Array.get a i)) (Expr.Var (Array.get b i)))
-            (Expr.Var (Array.get inv_marker i)))
-      )
-      (Lists.List.seq 0 (Z.to_nat NUM_LIMBS))
-      cmp_eq in
+    sum_for_in_zero_to_n_starting_from NUM_LIMBS (fun i =>
+      Expr.Mul
+        (Expr.Sub (Expr.Var (Array.get a i)) (Expr.Var (Array.get b i)))
+        (Expr.Var (Array.get inv_marker i))
+    ) cmp_eq in
   let! _ := MExpr.when is_valid (MExpr.assert_one sum) in
 
   let flags_with_opcode_integer : list (Var.t * Z) :=
@@ -148,21 +181,65 @@ Compute print_branch_eq (NUM_LIMBS := 4).
 
 (** We prove the equality of the [eval] definition above with the [eval] definition directly using
     field elements. *)
-Lemma eq_eval_field {p} `{Prime p} {NUM_LIMBS : Z}
-    (expr_env : Expr.Env.t)
-    (var_env : Var.Env.t)
+Lemma eval_eq {p} `{Prime p} {NUM_LIMBS : Z}
+    (env : Env.t)
     (self : BranchEqualCoreAir.t NUM_LIMBS)
     (local : BranchEqualCoreCols.t NUM_LIMBS Var.t)
     (from_pc : Var.t) :
-  MExpr.eval expr_env var_env (
-    MExpr.map (AdapterAirContext.map (Expr.eval expr_env var_env)) (
-      eval self local from_pc
-    )
-  ) =
-  core_with_monad.eval
-    self
-    (BranchEqualCoreCols.map (Var.eval var_env) local)
-    (Var.eval var_env from_pc).
+  MExpr.Eq.t env
+    (eval self local from_pc)
+    (core_with_monad.eval
+      self
+      (BranchEqualCoreCols.map (Var.eval env.(Env.var)) local)
+      (Var.eval env.(Env.var) from_pc)
+    ).
 Proof.
-  (* This lemma is not actually correct as the intermediates [Let] do not have the same type *)
-Admitted.
+  unfold eval, core_with_monad.eval.
+  econstructor. {
+    apply List.Eq.fold_left_eq; try reflexivity.
+    econstructor. {
+      repeat constructor.
+      cbn; now autorewrite with field_rewrite.
+    }
+    intros.
+    repeat constructor.
+  }
+  intros.
+  econstructor. {
+    constructor; cbn; now autorewrite with field_rewrite.
+  }
+  intros.
+  econstructor. {
+    constructor; cbn; now autorewrite with field_rewrite.
+  }
+  intros.
+  econstructor. {
+    apply MExpr.Eq.Pure.
+    unfold M.not.
+    now cbn; FieldRewrite.run.
+  }
+  intros.
+  econstructor. {
+    apply for_in_zero_to_n_eq.
+    intros.
+    now constructor.
+  }
+  intros.
+  econstructor. {
+    econstructor; try reflexivity.
+    constructor; try reflexivity.
+    cbn; autorewrite with field_rewrite.
+    f_equal.
+    now apply sum_for_in_zero_to_n_starting_from_eq.
+  }
+  intros.
+  constructor.
+  cbn; unfold AdapterAirContext.map; cbn.
+  f_equal.
+  { unfold M.not.
+    now cbn; FieldRewrite.run.
+  }
+  { unfold ImmInstruction.map; cbn; f_equal.
+    now cbn; FieldRewrite.run.
+  }
+Qed.
